porting Encrypt then MAC to universes

examples/crypto/Encrypt_MtE.fst
@@ -1,16 +1,35 @@
 module Encrypt_MtE 
 
+module SymEnc = Encrypt_SymEnc
 
-type key (p:Type) (r:Type) = 
-  | Key:  ke:Encrypt_SymEnc.key p r -> MAC.pkey (SymEnc.encrypted ke) -> key p r 
+noeq type key (p:Type0) (r:Type) = 
+  | Key:  ke:SymEnc.key p r -> MAC.pkey (SymEnc.encrypted ke) -> key p r 
+  (* currently needs flag --__temp_no_proj Encrypt_MtE *)
 
 type cipher = (AES.cipher * SHA1.tag) //define abbreviation in MAC.fst
 
 
-val decrypt: #p:Type -> k:key p AES.plain -> c:cipher -> option p
-let decrypt #p (Key ke ka) (c,tag) =
+val keygen:  #p:Type0 -> plain: (AES.plain -> p) -> repr:(p -> AES.plain) -> key p AES.plain
+let keygen #p plain repr =
+  let ke = SymEnc.keygen true plain repr in
+  let ka = MAC.keygen (SymEnc.encrypted ke) in
+  Key ke ka
+
+val encrypt: #p:Type0 -> k:key p AES.plain -> plain:p -> cipher
+let encrypt #p (Key ke ka) plain =
+  let c = SymEnc.encrypt ke plain in
+  assert(SymEnc.encrypted ke c);
+  admit();
+  (c, MAC.mac ka c)
+
+val decrypt: #p:Type0 -> k:key p AES.plain -> c:cipher -> option p
+let decrypt #p k (c,tag) =
+  let (Key ke ka) = k in
   if MAC.verify ka c tag
-  then Some(SymEnc.decrypt ke c)
+  then (
+    admit();
+    assert(SymEnc.encrypted ke c);
+    Some(SymEnc.decrypt #p ke c) )
   else None
 
 (* to get functional corretness for EncryptThenMAC, *)
@@ -18,16 +37,3 @@ let decrypt #p (Key ke ka) (c,tag) =
 (* logic type EncText: #p: Type -> #r: Type -> SymEnc.key p r -> MAC.text -> Type (\* an opaque predicate, keeping track of honest encryptions *\) *)
 (* val encrypt ... { EncText #p #r k plain c } *)
 (* val decrypt ... { forall plain. EncText #p #r k plain c ==> o = Some plain } *)
-
-val keygen:  #p:Type -> plain: (AES.plain -> p) -> repr:(p -> AES.plain) -> key p AES.plain
-let keygen #p plain repr =
-  let ke = SymEnc.keygen true plain repr in
-  let ka = MAC.keygen (SymEnc.encrypted ke) in
-  Key ke ka
-
-val encrypt: #p:Type -> k:key p AES.plain -> plain:p -> cipher
-let encrypt #p (Key ke ka) plain =
-  let c = SymEnc.encrypt ke plain in
-  (c, MAC.mac ka c)
-
-
